NTCB/SemanticsProp.v
@@ -1,0 +1,57 @@
+Require Import Lib.
+Require Import BinaryProps.
+Require Import Semantics.
+
+Module Type INSTRUCTION_SEMANTICS_PROP(Import I: INSTRUCTION).
+  (* the first parameter is to indicate that the n first bytes of the memory
+     cannot be written *)
+
+
+  (* an instruction cannot write in the lower code segment *)
+  Parameter sem_no_overwrite: forall code_segment_size instr st1 st2,
+    instruction_semantics code_segment_size instr st1 (Good_state st2) ->
+    forall n', n' < code_segment_size -> st1.(state_mem) n' = st2.(state_mem) n'.
+
+  (* the "good" instructions can get stuck but neverr lead to a "bad state" *)
+
+  Parameter sem_not_invalid_not_bad: forall instr,
+    classify_instruction instr <> Invalid_instruction ->
+    forall code_segment_size st tst,
+      instruction_semantics code_segment_size instr st tst ->
+      is_good_state tst.
+
+
+  Parameter sem_OK_instr_pc: forall bm instr size,
+    parse_instruction bm = Some (instr, size) ->
+    classify_instruction instr = OK_instr ->
+    forall code_segment_size st1 st2,
+    instruction_semantics code_segment_size instr st1 (Good_state st2) ->
+    st2.(state_pc) = st1.(state_pc) + (N_of_nat size).
+
+  Parameter sem_Mask_instr_pc: forall bm instr size,
+    parse_instruction bm = Some (instr, size) ->
+    forall reg w,
+    classify_instruction instr = Mask_instr reg w->
+    forall code_segment_size st1 st2,
+    instruction_semantics code_segment_size instr st1 (Good_state st2) ->
+    st2.(state_pc) = st1.(state_pc) + (N_of_nat size).
+
+  Parameter sem_Direct_jump_pc: forall bm instr size,
+    parse_instruction bm = Some (instr, size) ->
+    forall w,
+    classify_instruction instr = Direct_jump w ->
+    forall code_segment_size st1 st2,
+    instruction_semantics code_segment_size instr st1 (Good_state st2) ->
+    st2.(state_pc) = st1.(state_pc) + (N_of_nat size) \/
+    st2.(state_pc) = word_to_N w.
+
+  Parameter sem_Indirect_jump_pc: forall bm instr size,
+    parse_instruction bm = Some (instr, size) ->
+    forall reg,
+    classify_instruction instr = Indirect_jump reg ->
+    forall code_segment_size st1 st2,
+    instruction_semantics code_segment_size instr st1 (Good_state st2) ->
+    st2.(state_pc) = st1.(state_pc) + (N_of_nat size) \/
+    st2.(state_pc) = word_to_N (st1.(state_regs) reg).
+
+End INSTRUCTION_SEMANTICS_PROP.
