TCB/LazyList.v
@@ -1,0 +1,119 @@
+Require Import Lib.
+Set Implicit Arguments.
+Require Import BinaryProps.
+CoInductive lazy (X:Type) :=
+| Lazy : X -> lazy X.
+Implicit Arguments Lazy [[X]].
+
+Unset Elimination Schemes.
+
+Inductive lazy_list (X:Type) :=
+| ll_nil: lazy_list X
+| ll_cons: forall (x:X) (l: lazy (lazy_list X)), lazy_list X.
+
+Implicit Arguments ll_nil [[X]].
+Implicit Arguments ll_cons [[X]].
+
+Notation "x ::: ll" := (ll_cons x (Lazy ll)) (at level 60, right associativity).
+
+Notation "〈 〉" := (ll_nil).
+
+Notation "〈 x ; .. ; z 〉" := (ll_cons x (Lazy ( .. (ll_cons z (Lazy ll_nil)) .. ))).
+
+
+Set Elimination Schemes.
+
+Fixpoint lazy_list_rect (A:Type) (P : lazy_list A -> Type) (Hnil: P ll_nil)
+  (Hcons: forall (a: A) ll, P ll -> P (ll_cons a (Lazy ll))) (l: lazy_list A) : P l :=
+  match l as l0 return P l0 with
+    | 〈〉 => Hnil
+    | x ::: l' => (Hcons x l' (lazy_list_rect P Hnil Hcons l'))
+  end.
+
+Implicit Arguments lazy_list_rect [A].
+
+Definition lazy_list_ind (A:Type) (P : lazy_list A -> Prop) (Hnil: P ll_nil)
+  (Hcons: forall (a: A) ll, P ll -> P (ll_cons a (Lazy ll))) (l: lazy_list A) : P l :=
+  lazy_list_rect P Hnil Hcons l.
+
+Fixpoint to_list {X} (ll: lazy_list X) : list X :=
+  match ll with
+    | 〈〉 => []
+    | x ::: l' => x :: to_list l'
+  end.
+
+Fixpoint ll_length {X} (l: lazy_list X) : nat :=
+  match l with
+    | 〈〉 => O
+    | x ::: l' => S (ll_length l')
+  end.
+
+Lemma ll_length_correct: forall {X} (ll: lazy_list X),
+  ll_length ll = length (to_list ll).
+Proof.
+  induction ll; simpl; congruence.
+Qed.
+
+
+Fixpoint ll_nth {X} n (ll: lazy_list X) :=
+  match n, ll with
+    | _ ,〈〉 => None
+    | O, x ::: _ => Some x
+    | S n', _ ::: ll' => ll_nth n' ll'
+  end.
+
+Lemma ll_nth_correct: forall {X} n (ll: lazy_list X),
+  ll_nth n ll = nth_error (to_list ll) n.
+Proof.
+  induction n; simpl; intros; destruct ll as [| x [ll'] ]; simpl; auto.
+Qed.
+
+Fixpoint ll_safe_drop {X} (n: nat) (ll: lazy_list X) :=
+  match n with
+    | O => Some ll
+    | S n' =>
+      match ll with
+        | 〈〉 => None
+        | x ::: ll' => ll_safe_drop n' ll'
+      end
+  end.
+
+Lemma ll_safe_drop_size {X} n: forall  (ll ll': lazy_list X),
+  ll_safe_drop n ll = Some ll' ->
+  ll_length ll = (n + ll_length ll')%nat.
+Proof.
+  induction' n as [|n]; simpl; intros; clean.
+  Case "S n".
+  destruct ll as [| ? [ll2]]; clean.
+  specialize (IHn _ _ H).
+  simpl in *. congruence.
+Qed.
+
+
+Definition byte_map := nat -> option byte.
+Definition eq_byte_map (bm1 bm2: byte_map) := forall n, bm1 n = bm2 n.
+Notation "bm1 ≡ bm2" := (eq_byte_map bm1 bm2) (at level 70, no associativity).
+
+
+Definition start_map_from (start: nat) (bm: byte_map) : byte_map :=
+  fun n => bm (start + n)%nat.
+
+Lemma start_map_from_0: forall bm, start_map_from 0 bm ≡ bm.
+Proof.
+  intros bm n.
+  unfold start_map_from. simpl. reflexivity.
+Qed.
+
+Lemma start_map_from_right: forall start bm n,
+  (start_map_from start bm n) = bm (n + start)%nat.
+Proof.
+  intros; simpl. unfold start_map_from. f_equal. omega.
+Qed.
+
+Definition update_byte_map (bm: byte_map) (loc:nat) (ob: option byte): byte_map :=
+  fun n =>
+    if eq_nat_dec n loc then ob else bm n.
+
+
+Definition byte_map_from_ll (ll: lazy_list byte) : byte_map:=
+  fun n => ll_nth n ll.
